lib/hst/Math.Lemmas.fst
@@ -3,150 +3,7 @@ module Math.Lemmas
 open FStar.Mul
 open Math.Axioms
 
-#set-options "--z3timeout 10"
-
-(** Lemmas about multiplication, division and modulo. **)
-(** This part focuses on the situation where          **)
-(** dividend: nat    divisor: pos                     **)
-(** TODO: add triggers for certain lemmas.            **)
-
-(* Lemma: Definition of euclidian division *)
-val euclidian_division_definition: a:nat -> b:pos ->
-    Lemma (a = (a / b) * b + (a % b))
-let euclidian_division_definition a b = ()
-
-(* Lemma: Propriety about modulo *)
-val modulo_range_lemma: a:int -> b:pos ->
-    Lemma (a % b >= 0 && a % b < b)
-let modulo_range_lemma a b = ()
-
-val small_modulo_lemma_1: a:nat -> b:pos ->
-    Lemma (requires a < b) (ensures a % b = a)
-let small_modulo_lemma_1 a b = ()
-val small_modulo_lemma_2: a:nat -> b:pos ->
-    Lemma (requires a % b = a) (ensures a < b)
-let small_modulo_lemma_2 a b = ()
-
-val small_division_lemma_1: a:nat -> b:pos ->
-    Lemma (requires a < b) (ensures a / b = 0)
-let small_division_lemma_1 a b = ()
-val small_division_lemma_2: a:nat -> b:pos ->
-    Lemma (requires a / b = 0) (ensures a < b)
-let small_division_lemma_2 a b = ()
-
-(* Lemma: Multiplication by a positive integer preserves order *)
-val multiplication_order_lemma: a:nat -> b:nat -> p:pos ->
-    Lemma (a >= b <==> a * p >= b * p)
-let multiplication_order_lemma a b p = ()
-
-(* Lemma: Propriety about multiplication after division *)
-val division_propriety: a:nat -> b:pos ->
-    Lemma (a - b < (a / b) * b && (a / b) * b <= a)
-let division_propriety a b = ()
-
-(* Internal lemmas for proving the definition of division *)
-private val division_definition_lemma_1: a:nat -> b:pos -> m:nat{a - b < m * b} ->
-    Lemma (m > (a / b) - 1)
-let division_definition_lemma_1 a b m = 
-  if (a / b) - 1 < 0 then () else begin
-    division_propriety a b;
-    multiplication_order_lemma m ((a / b) - 1) b
-  end
-private val division_definition_lemma_2: a:nat -> b:pos -> m:nat{m * b <= a} ->
-    Lemma (m < (a / b) + 1)
-let division_definition_lemma_2 a b m =
-  division_propriety a b;
-  multiplication_order_lemma ((a / b) + 1) m b
-
-(* Lemma: Definition of division *)
-val division_definition: a:nat -> b:pos -> m:nat{a - b < m * b && m * b <= a} ->
-    Lemma (m = a / b)
-let division_definition a b m =
-  division_definition_lemma_1 a b m;
-  division_definition_lemma_2 a b m
-  
-(* Lemma: (a * b) / b = a *)
-val multiple_division_lemma: a:nat -> b:pos -> Lemma ( (a * b) / b = a )
-let multiple_division_lemma a b = division_definition (a * b) b a
-
-(* Lemma: (a * b) % b = 0 *)
-val multiple_modulo_lemma: a:nat -> b:pos -> Lemma ( (a * b) % b = 0 )
-let multiple_modulo_lemma a b = multiple_division_lemma a b
-
-(* Lemma: Division distributivity under special condition *)
-val division_addition_lemma: a:nat -> b:pos -> n:nat ->
-    Lemma ( (a + n * b) / b = (a / b) + n )
-let division_addition_lemma a b n = division_definition (a + n * b) b ((a / b) + n)
-
-(* Lemma: Modulo distributivity *)
-val modulo_distributivity: a:nat -> b:nat -> c:pos ->
-    Lemma ( (a + b) % c = (a % c + b % c) % c )
-let modulo_distributivity a b c =
-  euclidian_division_definition a c;
-  euclidian_division_definition b c;
-  division_addition_lemma (a - (a / c) * c + b - (b / c) * c) c (a / c + b / c)
-
-(* Lemma: Modulo distributivity under special condition *)
-val modulo_addition_lemma: a:nat -> b:pos -> n:nat ->
-    Lemma ( (a + n * b) % b = a % b )
-let modulo_addition_lemma a b n =
-  modulo_distributivity a (n * b) b;
-  multiple_modulo_lemma n b
-
-(* Lemma: Divided by a product is equivalent to being divided one by one *)
-val division_multiplication_lemma: a:nat -> b:pos -> c:pos ->
-    Lemma ( a / (b * c) = (a / b) / c )
-let division_multiplication_lemma a b c =
-  if a / b <= c - 1 then begin
-    small_division_lemma_1 (a / b) c;
-    small_division_lemma_1 a (b * c)
-  end else begin
-    division_propriety (a / b) c;
-    multiplication_order_lemma (a / b) (((a / b) / c) * c) b;
-    multiplication_order_lemma (((a / b) / c) * c) ((a / b) - c) b;
-    cut( ((a / b) - c + 1) * b <= ((a / b) / c) * c * b );
-    cut( ((a / b) / c) * c * b <= (a / b) * b );
-    division_definition a (b * c) ((a / b) / c)
-  end
-
-(* Lemma: Propriety about modulo and division *)
-val modulo_division_lemma: a:nat -> b:pos -> c:pos ->
-    Lemma ( (a % (b * c)) / b = (a / b) % c )
-let modulo_division_lemma a b c =
-  division_addition_lemma (a - (a / (b * c)) * (b * c)) b ((a / (b * c)) * c);
-  assert( (a - (a / (b * c)) * (b * c)) / b = (a - (a / (b * c)) * (b * c) + ((a / (b * c)) * c) * b) / b - ((a / (b * c)) * c));
-  cut( (a - (a / (b * c)) * (b * c)) / b = a / b - ((a / (b * c)) * c));
-  euclidian_division_definition a (b * c);
-  division_multiplication_lemma a b c;
-  euclidian_division_definition (a / b) c
-
-val modulo_modulo_lemma: a:nat -> b:pos -> c:pos ->
-    Lemma ( (a % (b * c)) % b = a % b )
-let modulo_modulo_lemma a b c =
-  modulo_addition_lemma (a - (a / (b * c)) * (b * c)) b ((a / (b * c)) * c);
-  assert( ((a - (a / (b * c)) * (b * c)) + ((a / (b * c)) * c) * b) % b = (a - (a / (b * c)) * (b * c)) % b );
-  cut( a % b = (a - (a / (b * c)) * (b * c)) % b );
-  euclidian_division_definition a (b * c)
-  
-
-(** Old lemmas **)
-(* Lemma: mutiplying by a positive number yield a greater output than input *)
-val star_incr_axiom: a:nat -> b:pos -> Lemma (a * b >= a)
-let star_incr_axiom a b = if a = 0 then () else multiplication_order_lemma b 1 a
-
-(* Lemma: euclidian division on nats yield a smaller output than its input *)
-val slash_decr_axiom: a:nat -> b:pos -> Lemma (a / b <= a)
-let slash_decr_axiom a b =
-  euclidian_division_definition a b;
-  if a / b = 0 then () else multiplication_order_lemma b 1 (a / b)
-  
-(* Lemma: definition of the "b divides c" relation *)
-val slash_star_axiom: a:int -> b:pos -> c:nat ->
-    Lemma (requires (a * b = c)) (ensures (a = c / b))
-let slash_star_axiom a b c =
-  if a >= 0 then multiple_division_lemma a b
-  else multiple_division_lemma (-a) b
-
+(* Old Lemmas *)
 (* Lemma: definition of the euclidian division for nats *)
 val euclidian_div_axiom:
   a:nat -> b:pos ->
@@ -170,11 +27,25 @@ val distributivity_add_right:
 let distributivity_add_right a b c = ()
 
 (* Lemma: multiplication is left distributive over substraction *)
+val distributivity_sub_left:
+  a:int -> b:int -> c:int ->
+  Lemma (requires (True))
+ (ensures ( (a - b) * c = a * c - b * c ))
+let distributivity_sub_left a b c = ()
+
+(* Lemma: multiplication is right distributive over substraction *)
 val distributivity_sub_right:
   a:int -> b:int -> c:int ->
   Lemma (requires (True))
  (ensures ( a * (b - c) = a * b - a * c ))
 let distributivity_sub_right a b c = ()
+
+(* Lemma: multiplication is commutative *)
+val commutativity_mul:
+  a:int -> b:int -> c:int ->
+  Lemma (requires (True))
+  (ensures ( (a * b) * c = a * (b * c) ))
+let commutativity_mul a b c = ()
 
 (* Lemma: multiplication is commutative, hence parenthesizing is meaningless *)
 val paren_mul_left:
@@ -298,6 +169,188 @@ val neg_of_non_multiple_is_non_multiple: a:int -> b:pos -> Lemma
     (requires (a % b <> 0))
     (ensures ((-a) % b <> 0))
 let neg_of_non_multiple_is_non_multiple a b = neg_modulo a b
+    
+val nat_mul_1: a:nat -> b:nat -> Lemma (requires True) (ensures (a*b >= 0))
+let nat_mul_1 a b = ()
+
+(* Lemma : multiplying by a strictly positive value preserves strict inequalities *)
+val mul_pos_strict_incr: a:pos -> b:int -> c:pos -> Lemma (requires (b < c)) (ensures (a * b < a * c /\ b * a < c * a ))
+let mul_pos_strict_incr a b c = ()
+
+(* Lemma : multiplying by a positive value preserves inequalities *)
+val mul_incr : a:nat -> b:nat -> c:nat -> 
+		     Lemma 
+		       (requires ( b <= c))
+		       (ensures ( a * b <= a * c /\ b * a <= c * a))
+let mul_incr a b c = ()
+
+(* Lemma : loss of precision in euclidian division *)
+val multiply_fractions:
+  a:nat -> n:pos ->
+  Lemma
+    (requires (True))
+    (ensures ( n * ( a / n ) <= a ))
+let multiply_fractions a n =
+  (euclidian_div_axiom a n)
+
+(* Lemma : distributivity of minus over parenthesized sum *)
+val paren_sub: a:int -> b:int -> c:int -> Lemma ((a - (b + c) = a - b - c /\ a - (b - c) = a - b + c))
+let paren_sub a b c = ()
+
+val non_zero_nat_is_pos: i:nat -> Lemma (requires (i <> 0)) (ensures (i >= 1))
+let non_zero_nat_is_pos i = ()
+
+val non_zero_nat_is_pos_2: n:nat -> Lemma (requires (n<>0)) (ensures (n-1>=0))
+let non_zero_nat_is_pos_2 n = ()
+
+val nat_plus_nat_is_nat: n:nat -> m:nat -> Lemma (n+m>=0)
+let nat_plus_nat_is_nat n m = ()
+
+(** Lemmas about multiplication, division and modulo. **)
+(** This part focuses on the situation where          **)
+(** dividend: nat    divisor: pos                     **)
+(** TODO: add triggers for certain lemmas.            **)
+
+(* Lemma: Definition of euclidian division *)
+val euclidian_division_definition: a:nat -> b:pos ->
+    Lemma (a = (a / b) * b + a % b)
+let euclidian_division_definition a b = ()
+
+(* Lemma: Propriety about modulo *)
+val modulo_range_lemma: a:int -> b:pos ->
+    Lemma (a % b >= 0 && a % b < b)
+let modulo_range_lemma a b = ()
+
+val small_modulo_lemma_1: a:nat -> b:pos ->
+    Lemma (requires a < b) (ensures a % b = a)
+let small_modulo_lemma_1 a b = ()
+val small_modulo_lemma_2: a:nat -> b:pos ->
+    Lemma (requires a % b = a) (ensures a < b)
+let small_modulo_lemma_2 a b = ()
+
+val small_division_lemma_1: a:nat -> b:pos ->
+    Lemma (requires a < b) (ensures a / b = 0)
+let small_division_lemma_1 a b = ()
+val small_division_lemma_2: a:nat -> b:pos ->
+    Lemma (requires a / b = 0) (ensures a < b)
+let small_division_lemma_2 a b = ()
+
+(* Lemma: Multiplication by a positive integer preserves order *)
+val multiplication_order_lemma: a:nat -> b:nat -> p:pos ->
+    Lemma (a >= b <==> a * p >= b * p)
+let multiplication_order_lemma a b p = ()
+
+(* Lemma: Propriety about multiplication after division *)
+val division_propriety: a:nat -> b:pos ->
+    Lemma (a - b < (a / b) * b && (a / b) * b <= a)
+let division_propriety a b = ()
+
+(* Internal lemmas for proving the definition of division *)
+private val division_definition_lemma_1: a:nat -> b:pos -> m:nat{a - b < m * b} ->
+    Lemma (m > a / b - 1)
+let division_definition_lemma_1 a b m = 
+  if a / b - 1 < 0 then () else begin
+    division_propriety a b;
+    multiplication_order_lemma m (a / b - 1) b
+  end
+private val division_definition_lemma_2: a:nat -> b:pos -> m:nat{m * b <= a} ->
+    Lemma (m < a / b + 1)
+let division_definition_lemma_2 a b m =
+  division_propriety a b;
+  multiplication_order_lemma (a / b + 1) m b
+
+(* Lemma: Definition of division *)
+val division_definition: a:nat -> b:pos -> m:nat{a - b < m * b && m * b <= a} ->
+    Lemma (m = a / b)
+let division_definition a b m =
+  division_definition_lemma_1 a b m;
+  division_definition_lemma_2 a b m
+  
+(* Lemma: (a * b) / b = a *)
+val multiple_division_lemma: a:nat -> b:pos -> Lemma ( (a * b) / b = a )
+let multiple_division_lemma a b = division_definition (a * b) b a
+
+(* Lemma: (a * b) % b = 0 *)
+val multiple_modulo_lemma: a:nat -> b:pos -> Lemma ( (a * b) % b = 0 )
+let multiple_modulo_lemma a b = multiple_division_lemma a b
+
+(* Lemma: Division distributivity under special condition *)
+val division_addition_lemma: a:nat -> b:pos -> n:nat ->
+    Lemma ( (a + n * b) / b = a / b + n )
+let division_addition_lemma a b n = division_definition (a + n * b) b (a / b + n)
+
+(* Lemma: Modulo distributivity *)
+val modulo_distributivity: a:nat -> b:nat -> c:pos ->
+    Lemma ( (a + b) % c = (a % c + b % c) % c )
+let modulo_distributivity a b c =
+  euclidian_division_definition a c;
+  euclidian_division_definition b c;
+  euclidian_division_definition (a % c + b % c) c;
+  nat_over_pos_is_nat a c;
+  nat_over_pos_is_nat b c;
+  division_addition_lemma (a - (a / c) * c + b - (b / c) * c) c (a / c + b / c)
+
+(* Lemma: Modulo distributivity under special condition *)
+val modulo_addition_lemma: a:nat -> b:pos -> n:nat ->
+    Lemma ( (a + n * b) % b = a % b )
+let modulo_addition_lemma a b n =
+  modulo_distributivity a (n * b) b;
+  multiple_modulo_lemma n b
+
+(* Lemma: Divided by a product is equivalent to being divided one by one *)
+val division_multiplication_lemma: a:nat -> b:pos -> c:pos ->
+    Lemma ( a / (b * c) = (a / b) / c )
+let division_multiplication_lemma a b c =
+  if a / b <= c - 1 then begin
+    small_division_lemma_1 (a / b) c;
+    small_division_lemma_1 a (b * c)
+  end else begin
+    division_propriety (a / b) c;
+    multiplication_order_lemma (a / b) (((a / b) / c) * c) b;
+    multiplication_order_lemma (((a / b) / c) * c) ((a / b) - c) b;
+    cut( ((a / b) - c + 1) * b <= (((a / b) / c) * c) * b );
+    cut( (((a / b) / c) * c) * b <= (a / b) * b );
+    nat_over_pos_is_nat a b;
+    nat_over_pos_is_nat (a / b) c;
+    division_definition a (b * c) ((a / b) / c)
+  end
+
+(* Lemma: Propriety about modulo and division *)
+val modulo_division_lemma: a:nat -> b:pos -> c:pos ->
+    Lemma ( (a % (b * c)) / b = (a / b) % c )
+let modulo_division_lemma a b c =
+  division_addition_lemma (a - (a / (b * c)) * (b * c)) b ((a / (b * c)) * c);
+  distributivity_sub_left a (a / (b * c)) (b * c);
+  commutativity_mul (a / (b * c)) c b;
+  cut( (a - (a / (b * c)) * (b * c)) / b = a / b - ((a / (b * c)) * c));
+  euclidian_division_definition a (b * c);
+  division_multiplication_lemma a b c;
+  euclidian_division_definition (a / b) c
+
+val modulo_modulo_lemma: a:nat -> b:pos -> c:pos ->
+    Lemma ( (a % (b * c)) % b = a % b )
+let modulo_modulo_lemma a b c =
+  modulo_addition_lemma (a - (a / (b * c)) * (b * c)) b ((a / (b * c)) * c);
+  assert( ((a - (a / (b * c)) * (b * c)) + ((a / (b * c)) * c) * b) % b = (a - (a / (b * c)) * (b * c)) % b );
+  cut( a % b = (a - (a / (b * c)) * (b * c)) % b );
+  euclidian_division_definition a (b * c)
+
+(* Lemma: mutiplying by a positive number yield a greater output than input *)
+val star_incr_axiom: a:nat -> b:pos -> Lemma (a * b >= a)
+let star_incr_axiom a b = if a = 0 then () else multiplication_order_lemma b 1 a
+
+(* Lemma: euclidian division on nats yield a smaller output than its input *)
+val slash_decr_axiom: a:nat -> b:pos -> Lemma (a / b <= a)
+let slash_decr_axiom a b =
+  euclidian_division_definition a b;
+  if a / b = 0 then () else multiplication_order_lemma b 1 (a / b)
+  
+(* Lemma: definition of the "b divides c" relation *)
+val slash_star_axiom: a:int -> b:pos -> c:nat ->
+    Lemma (requires (a * b = c)) (ensures (a = c / b))
+let slash_star_axiom a b c =
+  if a >= 0 then multiple_division_lemma a b
+  else multiple_division_lemma (-a) b
 
 val pow2_double_sum:
   n:nat -> Lemma (requires (True)) (ensures (pow2 n + pow2 n = pow2 (n+1))) 
@@ -366,39 +419,10 @@ let rec pow2_exp_1 n m =
     paren_mul_left 2 (pow2 (n-1)) (pow2 m);
     paren_mul_right 2 (pow2 (n-1)) (pow2 m);
     pow2_double_mult (n-1)
-    
-val nat_mul_1: a:nat -> b:nat -> Lemma (requires True) (ensures (a*b >= 0))
-let nat_mul_1 a b = ()
 
-(* Lemma : multiplying by a strictly positive value preserves strict inequalities *)
-val mul_pos_strict_incr: a:pos -> b:int -> c:pos -> Lemma (requires (b < c)) (ensures (a * b < a * c /\ b * a < c * a ))
-let mul_pos_strict_incr a b c = ()
-
-(* Lemma : multiplying by a positive value preserves inequalities *)
-val mul_incr : a:nat -> b:nat -> c:nat -> 
-		     Lemma 
-		       (requires ( b <= c))
-		       (ensures ( a * b <= a * c /\ b * a <= c * a))
-let mul_incr a b c = ()
-
-(* Lemma : loss of precision in euclidian division *)
-val multiply_fractions:
-  a:nat -> n:pos ->
-  Lemma
-    (requires (True))
-    (ensures ( n * ( a / n ) <= a ))
-let multiply_fractions a n =
-  (euclidian_div_axiom a n)
-
-(* Lemma : distributivity of minus over parenthesized sum *)
-val paren_sub: a:int -> b:int -> c:int -> Lemma ((a - (b + c) = a - b - c /\ a - (b - c) = a - b + c))
-let paren_sub a b c = ()
-
-val non_zero_nat_is_pos: i:nat -> Lemma (requires (i <> 0)) (ensures (i >= 1))
-let non_zero_nat_is_pos i = ()
-
-val non_zero_nat_is_pos_2: n:nat -> Lemma (requires (n<>0)) (ensures (n-1>=0))
-let non_zero_nat_is_pos_2 n = ()
-
-val nat_plus_nat_is_nat: n:nat -> m:nat -> Lemma (n+m>=0)
-let nat_plus_nat_is_nat n m = ()
+val pow2_exp_2: n:nat -> m:nat{m <= n} ->
+  Lemma (requires True)
+        (ensures pow2 n / pow2 m = pow2 (n - m))
+let pow2_exp_2 n m =
+  pow2_exp_1 m (n - m);
+  multiple_division_lemma (pow2 (n - m)) (pow2 m)
